Std/Data/OrderedAssocList.lean
@@ -1,0 +1,919 @@
+/-
+Copyright (c) 2023 Lean FRO, LLC. All rights reserved.
+Released under Apache 2.0 license as described in the file LICENSE.
+Authors: Scott Morrison
+-/
+import Std.Data.AssocList
+import Std.Classes.Order
+import Std.Data.Option.Lemmas
+import Std.Tactic.Ext
+import Std.Tactic.LeftRight
+import Std.Tactic.Omega
+
+/-!
+# Ordered association lists
+
+`OrderedAssocList` is a wrapper around `AssocList`,
+with the additional invariant that the keys are in strictly increasing order.
+
+As a consequence, an `OrderedAssocList` is determined by the `find?` function, that is
+`(∀ a, l₁.find? a = l₂.find? a) → l₁ = l₂`
+and this makes providing identities between operations more plausible than with `AssocList`.
+
+We will later add another wrapper requiring that a "default" value does not appear,
+so e.g. finitely supported functions can be uniquely represented.
+
+The main operations defined are:
+* `find?`, which linearly searches the list, stopping if the keys get too large.
+* `insert`, which inserts a new key-value pair, maintaining the order invariant.
+* `filterMapVal f`, for `f : α → β → Option γ`, which applies a function to values,
+  dropping some values.
+* `merge f` for `f : α → Option β → Option γ → Option δ` which merges two lists,
+  dropping some values. It runs in time `O(l₁.length + l₂.length)`.
+-/
+
+namespace Std
+
+/-!
+We first define some predicates and operations in the `AssocList` namespace.
+
+* `keysOrdered cmp l` asserts that the keys of an `l : AssocList` are strictly increasing
+  with respect to a comparator `cmp`.
+* `ltHeadKey? cmp a l` asserts that `a` is less than (according to `cmp`) the first key of `l`,
+  or that `l` is empty.
+-/
+
+namespace AssocList
+
+/--
+The predicate that the keys of an `AssocList` are
+in strictly increasing order according to the comparator `cmp`.
+-/
+def keysOrdered (cmp : α → α → Ordering) : AssocList α β → Prop
+  | .nil => True
+  | .cons _ _ .nil => True
+  | .cons a _ (.cons x y t) => cmp a x = .lt ∧ keysOrdered cmp (.cons x y t)
+
+instance instKeysOrderedDecidablePred : DecidablePred (keysOrdered cmp : AssocList α β → Prop) := by
+  rintro (_|⟨a, b, _|_⟩) <;> dsimp [keysOrdered]
+  · infer_instance
+  · infer_instance
+  · exact @instDecidableAnd _ _ _ (instKeysOrderedDecidablePred _)
+
+theorem keysOrdered.tail (h : keysOrdered cmp (.cons a b t)) : keysOrdered cmp t :=
+  match t with
+  | .nil => trivial
+  | .cons .. => h.2
+
+/-- The head key of an `AssocList`, or `none` if the list is empty. -/
+def headKey? (l : AssocList α β) : Option α :=
+  match l with
+  | .nil => none
+  | .cons a _ _ => some a
+
+@[simp] theorem headKey?_nil : headKey? (.nil : AssocList α β) = none := rfl
+@[simp] theorem headKey?_cons : headKey? (.cons a b t) = some a := rfl
+
+/--
+The condition that an element is less than the first key of an `AssocList`, or that list is empty.
+-/
+abbrev ltHeadKey? (cmp : α → α → Ordering) (a : α) (t : AssocList α β) : Prop :=
+  match headKey? t with | none => True | some x => cmp a x = .lt
+
+@[simp] theorem ltHeadKey?_nil {cmp : α → α → Ordering} :
+    ltHeadKey? cmp a (.nil : AssocList α β) = True := rfl
+@[simp] theorem ltHeadKey?_cons : ltHeadKey? cmp a (.cons x y t) = (cmp a x = .lt) := rfl
+
+theorem ltHeadKey?_of_keysOrdered_cons (w : keysOrdered cmp (cons a b t)) : ltHeadKey? cmp a t :=
+  match t with
+  | .nil => trivial
+  | .cons _ _ _ => w.1
+
+theorem ltHeadKey?_of_cons [TransCmp cmp] (w : ltHeadKey? cmp a (cons x y t))
+    (h : keysOrdered cmp (cons x y t)) :
+    ltHeadKey? cmp a t := by
+  have h := ltHeadKey?_of_keysOrdered_cons h
+  revert w h
+  dsimp [ltHeadKey?]
+  split
+  · simp
+  · exact TransCmp.lt_trans
+
+theorem ltHeadKey?_of_le [TransCmp cmp] (h : cmp x a ≠ .gt) (w : ltHeadKey? cmp a t) :
+    ltHeadKey? cmp x t := by
+  revert w
+  dsimp [ltHeadKey?]
+  split
+  · simp
+  · exact TransCmp.le_lt_trans h
+
+/--
+The head key of the first list is at most the head key of the second list,
+or the second list is empty.
+-/
+abbrev headKey?_le_headKey? (cmp : α → α → Ordering) (s : AssocList α β) (t : AssocList α γ) : Prop :=
+  match s.headKey?, t.headKey? with
+  | some a₁, some a₂ => cmp a₁ a₂ ≠ .gt
+  | none, some _ => False
+  | _, none => True
+
+@[simp] theorem headKey?_le_headKey?_cons_cons :
+    headKey?_le_headKey? cmp (cons a b t) (cons x y s) = (cmp a x ≠ .gt) := rfl
+
+theorem ltHeadKey?_of_headKey?_le_headKey? [TransCmp cmp]
+    (w : ltHeadKey? cmp a s) (h : headKey?_le_headKey? cmp s t) :
+    ltHeadKey? cmp a t := by
+  dsimp [ltHeadKey?, headKey?_le_headKey?] at *
+  revert h w
+  match headKey? s, headKey? t with
+  | some a, some b => exact TransCmp.lt_le_trans
+  | some a, none => intros; trivial
+  | none, some b => simp
+  | none, none => intros; trivial
+
+theorem headKey?_le_headKey?_cons [TransCmp cmp]
+    (h : keysOrdered cmp (cons x y t)) (w : headKey?_le_headKey? cmp t s) :
+    headKey?_le_headKey? cmp (cons x y t) s := by
+  have p := ltHeadKey?_of_keysOrdered_cons h
+  dsimp [ltHeadKey?, headKey?_le_headKey?] at *
+  revert p w
+  match headKey? s, headKey? t with
+  | some a, some b =>
+    intro p w
+    simp [TransCmp.lt_le_trans w p]
+  | some a, none => intros; trivial
+  | none, some b => simp
+  | none, none => intros; trivial
+
+theorem keysOrdered_cons {cmp : α → α → Ordering}
+    (w : ltHeadKey? cmp a t) (h : keysOrdered cmp t) :
+    keysOrdered cmp (.cons a b t) := by
+  match t with
+  | .nil => trivial
+  | .cons x y s => exact ⟨w, h⟩
+
+theorem find?_eq_none_of_ltHeadKey? {cmp : α → α → Ordering} [TransCmp cmp] [BEq α] [LawfulBEq α]
+    (w : ltHeadKey? cmp a l) (h : keysOrdered cmp l) :
+    l.find? a = none := by
+  match l with
+  | nil => rfl
+  | cons x y t =>
+    rw [find?]
+    split
+    · simp_all [OrientedCmp.cmp_refl]
+    · exact find?_eq_none_of_ltHeadKey? (ltHeadKey?_of_cons w h) h.tail
+
+/-!
+# Ordered-respecting operations on `AssocList`
+
+We now define `orderedInsert`, and `orderedMerge`,
+which will later be wrapped as `OrderedAssocList.insert` and `OrderedAssocList.merge`.
+
+We prove that with `keysOrdered` input these functions produce `keysOrdered` outputs.
+We prove that same about `AssocList.filterMapVal`.
+-/
+
+/--
+Insert a key-value pair into an `AssocList`,
+in such a way that if the original list has keys in increasing order,
+so does the result.
+(Otherwise, it is inserted before the first key the new key is smaller than,
+or replaces the first key the new key is equal to.)
+
+We later wrap this as `OrderedAssocList.insert`.
+-/
+def orderedInsert (cmp : α → α → Ordering) (l : AssocList α β) (a : α) (b : β) : AssocList α β :=
+  match l with
+  | .nil => .cons a b .nil
+  | .cons x y t => match w : cmp a x with
+    | .lt => .cons a b l
+    | .eq => .cons a b t
+    | .gt => .cons x y (orderedInsert cmp t a b)
+
+theorem headKey?_orderedInsert {l : AssocList α β} :
+    headKey? (orderedInsert cmp l a b) =
+      match headKey? l with
+        | none => some a
+        | some x => match cmp a x with | .lt | .eq => some a | .gt => some x := by
+  match l with
+  | .nil => rfl
+  | .cons x _ _ => dsimp [headKey?, orderedInsert]; cases cmp a x <;> rfl
+
+theorem headKey?_orderedInsert_or (cmp) (l : AssocList α β) (a) (b) :
+    headKey? (orderedInsert cmp l a b) = some a ∨
+      headKey? (orderedInsert cmp l a b) = headKey? l := by
+  rw [headKey?_orderedInsert]
+  match l with
+  | .nil => left; rfl
+  | .cons x y s => dsimp; cases cmp a x <;> simp
+
+theorem orderedInsert_keysOrdered [AntisymmCmp cmp] [OrientedCmp cmp] (h : keysOrdered cmp l) :
+    keysOrdered cmp (orderedInsert cmp l a b) := by
+  match l with
+  | .nil => trivial
+  | .cons x y t =>
+    dsimp [orderedInsert]
+    match w : cmp a x with
+    | .lt => exact ⟨w, h⟩
+    | .eq =>
+      rcases AntisymmCmp.eq_of_cmp_eq w with rfl
+      cases t <;> exact h
+    | .gt => exact aux h w
+-- I've split this step out with a name as it is useful to fill in a proof term later.
+where aux [AntisymmCmp cmp] [OrientedCmp cmp] {x y t}
+    (h : keysOrdered cmp (cons x y t)) (w : cmp a x = Ordering.gt) :
+    keysOrdered cmp (cons x y (orderedInsert cmp t a b)) := by
+        apply keysOrdered_cons
+        · dsimp [ltHeadKey?]
+          rcases headKey?_orderedInsert_or cmp t a b with (p|p)
+          · rw [p]
+            exact OrientedCmp.cmp_eq_gt.mp w
+          · rw [p]
+            exact ltHeadKey?_of_keysOrdered_cons h
+        · apply orderedInsert_keysOrdered
+          exact h.tail
+
+theorem headKey?_le_headKey?_filterMapVal [TransCmp cmp] (h : keysOrdered cmp l) :
+    headKey?_le_headKey? cmp l (l.filterMapVal f) := by
+  match l with
+  | .nil => simp [headKey?_le_headKey?]
+  | .cons x y t =>
+    simp [filterMapVal]
+    match f x y with
+    | none =>
+      exact headKey?_le_headKey?_cons h (headKey?_le_headKey?_filterMapVal h.tail)
+    | some _ => simp [OrientedCmp.cmp_refl]
+
+theorem filterMapVal_keysOrdered [TransCmp cmp] (h : keysOrdered cmp l) :
+    keysOrdered cmp (l.filterMapVal f) := by
+  match l with
+  | .nil => exact h
+  | .cons x y t =>
+    simp only [filterMapVal]
+    split
+    · exact filterMapVal_keysOrdered h.tail
+    · apply keysOrdered_cons
+      · exact ltHeadKey?_of_headKey?_le_headKey? (ltHeadKey?_of_keysOrdered_cons h)
+          (headKey?_le_headKey?_filterMapVal h.tail)
+      · exact filterMapVal_keysOrdered h.tail
+
+/--
+Merge two `AssocList`s,
+at each stage taking the first key-value pair from whichever list has a smaller first key.
+If both inputs have keys in strictly increasing order, so does the result.
+(We later wrap this as `OrderedAssocList.merge`.)
+
+We combine values using a function `f : α → Option β → Option γ → Option δ` which we call as
+`f a (some b) none` when encountering a key present only in the first list (with value `b`),
+`f a none (some g)` when encountering a key present only in the second list (with value `g`), and
+`f a (some b) (some g)` when encountering a key present in both lists.
+(Note the value of `f a none none` is never used.)
+-/
+def orderedMerge (cmp : α → α → Ordering) (f : α → Option β → Option γ → Option δ) :
+    AssocList α β → AssocList α γ → AssocList α δ
+  | .nil, .nil => nil
+  | .nil, .cons a₂ g t₂ => filterMapVal (fun a g => f a none (some g)) (.cons a₂ g t₂)
+  | .cons a₁ b t₁, .nil => filterMapVal (fun a b => f a (some b) none) (.cons a₁ b t₁)
+  | .cons a₁ b t₁, .cons a₂ g t₂ => match cmp a₁ a₂ with
+    | .lt => match (f a₁ (some b) none) with
+      | some d => .cons a₁ d (orderedMerge cmp f t₁ (.cons a₂ g t₂))
+      | none => orderedMerge cmp f t₁ (.cons a₂ g t₂)
+    | .eq => match (f a₁ (some b) (some g)) with
+      | some d => .cons a₁ d (orderedMerge cmp f t₁ t₂)
+      | none => orderedMerge cmp f t₁ t₂
+    | .gt => match (f a₂ none (some g)) with
+      | some d => .cons a₂ d (orderedMerge cmp f (.cons a₁ b t₁) t₂)
+      | none => orderedMerge cmp f (.cons a₁ b t₁) t₂
+termination_by _ l₁ l₂ => l₁.length + l₂.length
+decreasing_by simp_wf; omega
+
+theorem ltHeadKey?_orderedMerge [TransCmp cmp]
+    (h₁ : ltHeadKey? cmp a l₁) (h₂ : ltHeadKey? cmp a l₂)
+    (w₁ : keysOrdered cmp l₁) (w₂ : keysOrdered cmp l₂) :
+    ltHeadKey? cmp a (orderedMerge cmp f l₁ l₂) := by
+  match l₁, l₂ with
+  | .nil, .nil => simp [orderedMerge]
+  | .nil, .cons a₂ g t₂ =>
+    rw [orderedMerge]
+    exact ltHeadKey?_of_headKey?_le_headKey? h₂ (headKey?_le_headKey?_filterMapVal w₂)
+  | .cons a₁ b t₁, .nil =>
+    rw [orderedMerge]
+    exact ltHeadKey?_of_headKey?_le_headKey? h₁ (headKey?_le_headKey?_filterMapVal w₁)
+  | .cons a₁ b t₁, .cons a₂ g t₂ =>
+    rw [orderedMerge]
+    match cmp a₁ a₂ with
+    | .lt =>
+      dsimp
+      split
+      · exact h₁
+      · exact ltHeadKey?_orderedMerge (ltHeadKey?_of_cons h₁ w₁) h₂ w₁.tail w₂
+    | .eq =>
+      dsimp
+      split
+      · exact h₁
+      · exact ltHeadKey?_orderedMerge (ltHeadKey?_of_cons h₁ w₁) (ltHeadKey?_of_cons h₂ w₂)
+          w₁.tail w₂.tail
+    | .gt =>
+      dsimp
+      split
+      · exact h₂
+      · exact ltHeadKey?_orderedMerge h₁ (ltHeadKey?_of_cons h₂ w₂) w₁ w₂.tail
+
+theorem orderedMerge_keysOrdered [AntisymmCmp cmp] [TransCmp cmp]
+    (h₁ : keysOrdered cmp l₁) (h₂ : keysOrdered cmp l₂) :
+    keysOrdered cmp (orderedMerge cmp f l₁ l₂) := by
+  match l₁, l₂ with
+  | .nil, .nil => trivial
+  | .nil, .cons a₂ g t₂ => exact filterMapVal_keysOrdered h₂
+  | .cons a₁ b t₁, .nil => exact filterMapVal_keysOrdered h₁
+  | .cons a₁ b t₁, .cons a₂ g t₂ =>
+    rw [orderedMerge]
+    match h : cmp a₁ a₂ with
+    | .lt => match (f a₁ (some b) none) with
+      | some d =>
+        apply keysOrdered_cons
+        · apply ltHeadKey?_orderedMerge (ltHeadKey?_of_keysOrdered_cons h₁) (ltHeadKey?_cons.mpr h)
+            h₁.tail h₂
+        · exact orderedMerge_keysOrdered h₁.tail h₂
+      | none => exact orderedMerge_keysOrdered h₁.tail h₂
+    | .eq => match (f a₁ (some b) (some g)) with
+      | some d =>
+        dsimp
+        apply keysOrdered_cons
+        · rcases (AntisymmCmp.eq_of_cmp_eq h) with rfl
+          exact ltHeadKey?_orderedMerge (ltHeadKey?_of_keysOrdered_cons h₁)
+            (ltHeadKey?_of_keysOrdered_cons h₂) h₁.tail h₂.tail
+        · exact orderedMerge_keysOrdered h₁.tail h₂.tail
+      | none => exact orderedMerge_keysOrdered h₁.tail h₂.tail
+    | .gt => match (f a₂ none (some g)) with
+      | some d =>
+        apply keysOrdered_cons
+        · apply ltHeadKey?_orderedMerge (ltHeadKey?_cons.mpr (OrientedCmp.cmp_eq_gt.mp h))
+            (ltHeadKey?_of_keysOrdered_cons h₂) h₁ h₂.tail
+        · exact orderedMerge_keysOrdered h₁ h₂.tail
+      | none => exact orderedMerge_keysOrdered h₁ h₂.tail
+
+end AssocList
+
+/--
+An `OrderedAssocList` is an `AssocList` with the additional invariant that
+the keys are in strictly increasing order according to some specified comparator function.
+-/
+structure OrderedAssocList {α : Type u} (cmp : α → α → Ordering) (β : Type v) where
+  /-- The underlying `AssocList` of an `OrderedAssocList`. -/
+  list : AssocList α β
+  /-- The invariant that the keys are in strictly increasing order according to `cmp`. -/
+  keysOrdered : list.keysOrdered cmp
+
+namespace OrderedAssocList
+
+variable {α : Type u} {cmp : α → α → Ordering}
+
+/-- The empty `OrderedAssocList`. -/
+def nil : OrderedAssocList cmp β := ⟨.nil, trivial⟩
+
+/-- The length of an `OrderedAssocList`. -/
+def length (l : OrderedAssocList cmp β) : Nat := l.list.length
+
+@[simp] theorem length_nil : length (nil : OrderedAssocList cmp β) = 0 := rfl
+@[simp] theorem length_mk_cons : length ⟨.cons a b t, h⟩ = length ⟨t, h.tail⟩ + 1 :=
+  rfl
+
+/-- The first key-value pair in an `OrderedAssocList`. -/
+def head? (l : OrderedAssocList cmp β) : Option (α × β) :=
+  match l with
+  | ⟨.nil, _⟩ => none
+  | ⟨.cons a b _, _⟩ => some (a, b)
+
+/-- The tail of an `OrderedAssocList`. -/
+def tail (l : OrderedAssocList cmp β) : OrderedAssocList cmp β :=
+  match l with
+  | ⟨.nil, _⟩ => l
+  | ⟨.cons _ _ t, h⟩ => ⟨t, h.tail⟩
+
+@[simp] theorem length_tail : length (tail l) = length l - 1 := by
+  match l with
+  | ⟨.nil, _⟩ => rfl
+  | ⟨.cons _ _ _, _⟩ => rfl
+
+/--
+Find the value associated to a key by traversing left to right,
+short-circuiting once we are considering larger keys.
+-/
+def find? (l : OrderedAssocList cmp β) (x : α) : Option β :=
+  match l with
+  | ⟨.nil, _⟩ => none
+  | ⟨.cons a b t, h⟩ => match cmp x a with
+    | .lt => none
+    | .eq => some b
+    | .gt => find? ⟨t, h.tail⟩ x
+
+theorem find?_eq_find?_list [AntisymmCmp cmp] [TransCmp cmp] [BEq α] [LawfulBEq α]
+    {l : OrderedAssocList cmp β} : l.find? x = l.list.find? x := by
+  match l with
+  | ⟨.nil, _⟩ => rfl
+  | ⟨.cons a b t, h⟩ =>
+    rw [find?, AssocList.find?]
+    split
+    · split
+      · simp_all [OrientedCmp.cmp_refl]
+      · rw [AssocList.find?_eq_none_of_ltHeadKey? (cmp := cmp)]
+        · exact AssocList.ltHeadKey?_of_le (by simp_all)
+            (AssocList.ltHeadKey?_of_keysOrdered_cons h)
+        · exact h.tail
+    · simp_all [AntisymmCmp.eq_of_cmp_eq ‹_›]
+    · split
+      · simp_all [OrientedCmp.cmp_refl]
+      · apply find?_eq_find?_list
+
+@[simp] theorem find?_nil : find? (nil : OrderedAssocList cmp β) x = none := rfl
+@[simp] theorem find?_mk_nil : find? ⟨.nil, h⟩ x = none := rfl
+
+/-- The first key in an `OrderedAssocList`, or `none` if the list is empty. -/
+def headKey? (l : OrderedAssocList cmp β) : Option α := l.list.headKey?
+
+@[simp] theorem headKey?_nil : headKey? (nil : OrderedAssocList cmp β) = none := rfl
+@[simp] theorem headKey?_mk_cons : headKey? ⟨.cons a b t, h⟩ = some a := rfl
+
+/-- Either `a` is less than the first key of `l`, or `l` is empty. -/
+def ltHeadKey? (a : α) (l : OrderedAssocList cmp β) : Prop := AssocList.ltHeadKey? cmp a l.list
+
+/-- The head key of a tail is either `none`, or greater than the original head key. -/
+theorem headKey?_tail (h : AssocList.keysOrdered cmp (.cons a b t)) :
+    ltHeadKey? a ⟨t, h.tail⟩ := by
+  dsimp [ltHeadKey?]
+  match t with
+  | .nil => trivial
+  | .cons _ _ _ => exact h.1
+
+theorem find?_eq_none_of_ltHeadKey? (l : OrderedAssocList cmp β) (w : ltHeadKey? x l) :
+    find? l x = none := by
+  match l with
+  | ⟨.nil, _⟩ => rfl
+  | ⟨.cons a b t, h⟩ =>
+    match p : cmp x a with
+    | .lt => simp [find?, p]
+    | .eq => simp_all [ltHeadKey?]
+    | .gt => simp_all [ltHeadKey?]
+
+theorem find?_mk_cons [OrientedCmp cmp] [TransCmp cmp]
+    {h : (AssocList.cons a b t).keysOrdered cmp} :
+    find? ⟨.cons a b t, h⟩ x = if cmp x a = .eq then some b else find? ⟨t, h.tail⟩ x := by
+  simp only [find?]
+  split <;> rename_i w <;> simp only [w, ite_true, ite_false]
+  rw [find?_eq_none_of_ltHeadKey?]
+  have p := headKey?_tail h
+  revert p
+  simp only [ltHeadKey?, AssocList.ltHeadKey?]
+  split
+  · trivial
+  · exact TransCmp.lt_trans w
+
+@[simp] theorem find?_mk_cons_self [OrientedCmp cmp] {h : (AssocList.cons a b t).keysOrdered cmp} :
+    find? ⟨.cons a b t, h⟩ a = some b := by
+  simp [find?, OrientedCmp.cmp_refl]
+
+theorem ext_list {l₁ l₂ : OrderedAssocList cmp β} (w : l₁.list = l₂.list) : l₁ = l₂ := by
+  cases l₁; cases l₂; congr
+
+theorem ext [AntisymmCmp cmp] [OrientedCmp cmp] [TransCmp cmp] {l₁ l₂ : OrderedAssocList cmp β}
+    (w : ∀ a, l₁.find? a = l₂.find? a) : l₁ = l₂ := by
+  match h₁ : l₁, h₂ : l₂ with
+  | ⟨.nil, _⟩, ⟨.nil, _⟩ => rfl
+  | ⟨.cons a b t, _⟩, ⟨.nil, _⟩ =>
+    exfalso
+    specialize w a
+    simp_all
+  | ⟨.nil, _⟩, ⟨.cons a b t, _⟩ =>
+    exfalso
+    specialize w a
+    simp_all
+  | ⟨.cons a₁ b₁ t₁, p₁⟩, ⟨.cons a₂ b₂ t₂, p₂⟩ =>
+    match h : cmp a₁ a₂ with
+    | .lt =>
+      exfalso
+      have w₂ : l₂.find? a₁ = none := by
+        simp [find?_eq_none_of_ltHeadKey?, h₂, ltHeadKey?, h]
+      specialize w a₁
+      simp_all
+    | .eq =>
+      rcases AntisymmCmp.eq_of_cmp_eq h
+      have w' := w a₁
+      simp only [find?_mk_cons_self, Option.some.injEq] at w'
+      congr
+      suffices (⟨t₁, p₁.tail⟩ : OrderedAssocList cmp β) = ⟨t₂, p₂.tail⟩ by injections
+      apply ext
+      intro a
+      specialize w a
+      simp only [find?_mk_cons] at w
+      split at w <;> rename_i h
+      · rcases AntisymmCmp.eq_of_cmp_eq h
+        rw [find?_eq_none_of_ltHeadKey?, find?_eq_none_of_ltHeadKey?]
+        apply headKey?_tail p₂
+        apply headKey?_tail p₁
+      · exact w
+    | .gt =>
+      exfalso
+      have w₁ : l₁.find? a₂ = none := by
+        simp [find?_eq_none_of_ltHeadKey?, h₁, ltHeadKey?, h, ← OrientedCmp.cmp_eq_gt]
+      specialize w a₂
+      simp_all
+
+-- Since this was a recursive theorem we have to add the attribute after the fact.
+attribute [ext] ext
+
+/-- Check if an `OrderedAssocList` contains a specific key. -/
+def contains (l : OrderedAssocList cmp β) (x : α) : Bool := (l.find? x).isSome
+
+@[simp] theorem contains_nil : contains (nil : OrderedAssocList cmp β) x = false := rfl
+@[simp] theorem contains_mk_cons_self [OrientedCmp cmp]
+    {h : (AssocList.cons a b t).keysOrdered cmp} :
+    contains ⟨.cons a b t, h⟩ a = true := by
+  simp [contains]
+
+/--
+Prepend a key-value pair,
+requiring a proof that the key is smaller than the existing smallest key.
+-/
+def cons (a : α) (b : β) (l : OrderedAssocList cmp β) (w : ltHeadKey? a l) :
+    OrderedAssocList cmp β :=
+  match l with
+  | ⟨.nil, _⟩ => ⟨.cons a b .nil, trivial⟩
+  | ⟨.cons x y t, h⟩ => ⟨.cons a b (.cons x y t), ⟨w, h⟩⟩
+
+@[simp] theorem list_cons : (cons a b l w).list = .cons a b l.list := by
+  dsimp [cons]
+  match l with
+  | ⟨.nil, _⟩ => rfl
+  | ⟨.cons x y t, h⟩ => rfl
+
+@[simp] theorem find?_cons [TransCmp cmp] {l : OrderedAssocList cmp β} {w} :
+    (cons a b l w).find? x = if cmp x a = .eq then some b else l.find? x := by
+  simp only [cons]
+  split <;> simp [find?_mk_cons]
+
+@[simp] theorem headKey?_cons : headKey? (cons a b l w) = some a := by
+  match l with
+  | ⟨.nil, _⟩
+  | ⟨.cons _ _ _, _⟩ => rfl
+
+section insert
+variable [AntisymmCmp cmp]
+
+section
+variable [OrientedCmp cmp]
+
+/--
+Insert a key-value pair into an `OrderedAssocList`.
+This replaces the current value if the key is already present,
+and otherwise inserts it before the first key which is greater than the inserted key.
+-/
+def insert (l : OrderedAssocList cmp β) (a : α) (b : β) : OrderedAssocList cmp β :=
+  ⟨l.list.orderedInsert cmp a b, AssocList.orderedInsert_keysOrdered l.keysOrdered⟩
+
+@[simp] theorem insert_mk_nil :
+    insert (⟨.nil, h⟩ : OrderedAssocList cmp β) a b = ⟨.cons a b .nil, trivial⟩ := rfl
+
+@[simp] theorem insert_mk_cons :
+    insert (⟨.cons x y t, h⟩ : OrderedAssocList cmp β) a b = match w : cmp a x with
+    | .lt => ⟨.cons a b (.cons x y t), ⟨w, h⟩⟩
+    | .eq => ⟨.cons a b t, by
+        cases (AntisymmCmp.eq_of_cmp_eq w); cases t <;> exact h⟩
+    | .gt => .cons x y (insert ⟨t, h.tail⟩ a b) (AssocList.ltHeadKey?_of_keysOrdered_cons
+        (AssocList.orderedInsert_keysOrdered.aux h w)) := by
+  dsimp [insert, AssocList.orderedInsert]
+  congr
+  split <;> simp
+
+theorem length_insert_ne_zero {l : OrderedAssocList cmp β} : (insert l a b).length ≠ 0 := by
+  match l with
+  | ⟨.nil, _⟩ => simp
+  | ⟨.cons x y t, _⟩ =>
+    dsimp [insert, AssocList.orderedInsert, length]
+    split <;> simp
+
+end
+
+variable [TransCmp cmp]
+
+theorem find?_insert (l : OrderedAssocList cmp β) (a : α) (b : β) :
+    (insert l a b).find? x = if cmp x a = .eq then some b else l.find? x := by
+  match l with
+  | ⟨.nil, _⟩ => simp only [insert_mk_nil, find?_mk_cons]
+  | ⟨.cons a' b' t, h⟩ =>
+    simp only [insert_mk_cons]
+    split <;> rename_i h₁
+    · simp [find?_mk_cons]
+    · rcases AntisymmCmp.eq_of_cmp_eq h₁
+      simp [find?_mk_cons]
+    · rw [find?_cons, find?_insert ⟨t, h.tail⟩, find?_mk_cons]
+      split <;> rename_i h₂
+      · rcases (AntisymmCmp.eq_of_cmp_eq h₂).symm
+        simp_all [OrientedCmp.cmp_eq_gt]
+      · rfl
+termination_by _ => l.length
+
+theorem find?_insert_self (l : OrderedAssocList cmp β) (a : α) (b : β) :
+    (insert l a b).find? a = some b := by
+  simp [find?_insert, OrientedCmp.cmp_refl]
+
+theorem insert_contains (l : OrderedAssocList cmp β) (a : α) (b : β) :
+    (l.insert a b).contains x = ((cmp x a = .eq) || l.contains x) := by
+  simp only [contains, find?_insert]
+  split <;> rename_i h
+  · simp [h]
+  · cases find? l x <;> simp [h]
+
+theorem insert_contains_self (l : OrderedAssocList cmp β) (a : α) (b : β) :
+    (l.insert a b).contains a = true := by
+  simp [insert_contains, OrientedCmp.cmp_refl]
+
+end insert
+
+section filterMapVal
+
+variable [TransCmp cmp]
+
+/--
+Apply a function to each key-value pair,
+either replacing the value or dropping it if the function returns `none`.
+-/
+def filterMapVal (f : α → β → Option δ) (l : OrderedAssocList cmp β) :
+    OrderedAssocList cmp δ :=
+  ⟨l.list.filterMapVal f, AssocList.filterMapVal_keysOrdered l.keysOrdered⟩
+
+@[simp] theorem filterMapVal_nil {f : α → β → Option γ} :
+    filterMapVal f (nil : OrderedAssocList cmp β) = nil := rfl
+
+private theorem filterMapVal_mk_cons_list (f : α → β → Option γ) (x) (y) (t) (h) :
+    (filterMapVal f (⟨.cons x y t, h⟩ : OrderedAssocList cmp β)).list =
+      match f x y with
+      | none => AssocList.filterMapVal f t
+      | some g => .cons x g (filterMapVal f ⟨t, h.tail⟩).1 := by
+  dsimp [filterMapVal, AssocList.filterMapVal]
+  split <;> simp_all
+
+private theorem filterMapVal_mk_cons {f : α → β → Option γ} :
+    filterMapVal f (⟨.cons x y t, h⟩ : OrderedAssocList cmp β) =
+      match w : f x y with
+      | none => filterMapVal f ⟨t, h.tail⟩
+      | some g => ⟨.cons x g (filterMapVal f ⟨t, h.tail⟩).1, by
+          have p := filterMapVal_mk_cons_list f x y t h
+          simp only [w] at p
+          simp only [← p]
+          exact (filterMapVal f ⟨.cons x y t, h⟩).keysOrdered⟩ := by
+  apply ext_list
+  simp only [filterMapVal_mk_cons_list]
+  split <;> simp_all [filterMapVal]
+
+@[simp]
+theorem find?_filterMapVal [AntisymmCmp cmp] (l : OrderedAssocList cmp β) :
+    (filterMapVal f l).find? a = (l.find? a).bind (fun b => f a b) := by
+  -- This isn't true at the level of `AssocList`; we need uniqueness of keys.
+  match l with
+  | ⟨.nil, _⟩ => rfl
+  | ⟨.cons x y t, h⟩ =>
+    simp only [filterMapVal_mk_cons, find?_mk_cons]
+    split
+    · rw [find?_filterMapVal ⟨t, h.tail⟩]
+      split <;> rename_i h'
+      · have h' := AntisymmCmp.eq_of_cmp_eq h'
+        rw [find?_eq_none_of_ltHeadKey?]
+        · simp_all
+        · rcases h' with rfl
+          exact AssocList.ltHeadKey?_of_keysOrdered_cons h
+      · rfl
+    · simp only [find?_mk_cons]
+      split <;> rename_i h'
+      · simp_all [AntisymmCmp.eq_of_cmp_eq h']
+      · rw [find?_filterMapVal]
+termination_by _ l => l.length
+
+theorem filterMapVal_filterMapVal [AntisymmCmp cmp] [TransCmp cmp]
+    {f : α → γ → Option δ} {g : α → β → Option γ}
+    {l : OrderedAssocList cmp β} :
+    filterMapVal f (filterMapVal g l) = filterMapVal (fun a b => (g a b).bind (fun c => f a c)) l := by
+  ext a d
+  simp only [find?_filterMapVal, Option.mem_def, Option.bind_eq_some]
+  constructor
+  · rintro ⟨c, ⟨⟨b, hb, hc⟩, hd⟩⟩
+    refine ⟨b, hb, c, hc, hd⟩
+  · rintro ⟨b, hb, c, hc, hd⟩
+    refine ⟨c, ⟨⟨b, hb, hc⟩, hd⟩⟩
+
+end filterMapVal
+
+section merge
+
+variable [AntisymmCmp cmp] [TransCmp cmp]
+
+/--
+Merge two `OrderedAssocList`s using a function `α → Option β → Option γ → Option δ`,
+dropping values where the function returns `none`.
+-/
+def merge (f : α → Option β → Option γ → Option δ)
+    (l₁ : OrderedAssocList cmp β) (l₂ : OrderedAssocList cmp γ) : OrderedAssocList cmp δ :=
+  ⟨AssocList.orderedMerge cmp f l₁.list l₂.list,
+    AssocList.orderedMerge_keysOrdered l₁.keysOrdered l₂.keysOrdered⟩
+
+@[simp] theorem list_merge {l₁ : OrderedAssocList cmp β} :
+    (merge f l₁ l₂).list = AssocList.orderedMerge cmp f l₁.list l₂.list :=
+  rfl
+
+@[simp] theorem merge_nil_nil {f : α → Option β → Option γ → Option δ} :
+    merge f (nil : OrderedAssocList cmp β) nil = nil := rfl
+
+@[simp] theorem merge_mk_nil_mk_cons {f : α → Option β → Option γ → Option δ} :
+    merge f (⟨.nil, h⟩ : OrderedAssocList cmp β) ⟨.cons x' y' t', h'⟩ =
+      filterMapVal (fun a g => f a none (some g)) ⟨.cons x' y' t', h'⟩ := rfl
+
+@[simp] theorem merge_mk_cons_mk_nil {f : α → Option β → Option γ → Option δ} :
+    merge f ⟨.cons x y t, h⟩ (⟨.nil, h'⟩ : OrderedAssocList cmp γ) =
+      filterMapVal (fun a b => f a (some b) none) ⟨.cons x y t, h⟩ := rfl
+
+private theorem merge_mk_cons_mk_cons_list
+    (f : α → Option β → Option γ → Option δ) (x y t h x' y' t' h') :
+    (merge f (⟨.cons x y t, h⟩ : OrderedAssocList cmp β) ⟨.cons x' y' t', h'⟩).list =
+      match cmp x x' with
+      | .lt => match f x (some y) none with
+        | none => AssocList.orderedMerge cmp f t (.cons x' y' t')
+        | some d => .cons x d (AssocList.orderedMerge cmp f t (.cons x' y' t'))
+      | .eq => match f x (some y) (some y') with
+        | none => AssocList.orderedMerge cmp f t t'
+        | some d => .cons x d (AssocList.orderedMerge cmp f t t')
+      | .gt => match f x' none (some y') with
+        | none => AssocList.orderedMerge cmp f (.cons x y t) t'
+        | some d => .cons x' d (AssocList.orderedMerge cmp f (.cons x y t) t') := by
+  dsimp [merge]
+  rw [AssocList.orderedMerge]
+  split <;> split <;> simp_all
+
+private theorem merge_mk_cons_mk_cons {f : α → Option β → Option γ → Option δ} :
+    merge f (⟨.cons x y t, h⟩ : OrderedAssocList cmp β) ⟨.cons x' y' t', h'⟩ =
+      match i: cmp x x' with
+      | .lt => match w : f x (some y) none with
+        | none => merge f ⟨t, h.tail⟩ ⟨.cons x' y' t', h'⟩
+        | some d => ⟨.cons x d (merge f ⟨t, h.tail⟩ ⟨.cons x' y' t', h'⟩).list, by
+            have p := merge_mk_cons_mk_cons_list f x y t h x' y' t' h'
+            simp only [w, i] at p
+            simp only [list_merge]
+            simp only [← p]
+            exact (merge f _ _).keysOrdered⟩
+      | .eq => match w : f x (some y) (some y') with
+        | none => merge f ⟨t, h.tail⟩ ⟨t', h'.tail⟩
+        | some d => ⟨.cons x d (merge f ⟨t, h.tail⟩ ⟨t', h'.tail⟩).list, by
+            have p := merge_mk_cons_mk_cons_list f x y t h x' y' t' h'
+            simp only [w, i] at p
+            simp only [list_merge]
+            simp only [← p]
+            exact (merge f _ _).keysOrdered⟩
+      | .gt => match w : f x' none (some y') with
+        | none => merge f ⟨.cons x y t, h⟩ ⟨t', h'.tail⟩
+        | some d => ⟨.cons x' d (merge f ⟨.cons x y t, h⟩ ⟨t', h'.tail⟩).list, by
+            have p := merge_mk_cons_mk_cons_list f x y t h x' y' t' h'
+            simp only [w, i] at p
+            simp only [list_merge]
+            simp only [← p]
+            exact (merge f _ _).keysOrdered⟩ := by
+  apply ext_list
+  simp only [merge_mk_cons_mk_cons_list]
+  split <;> split <;> simp_all [merge]
+
+@[simp] theorem find?_merge {f : α → Option β → Option γ → Option δ}
+    (hf : f a none none = none) {l₁ : OrderedAssocList cmp β} {l₂} :
+    (merge f l₁ l₂).find? a = f a (l₁.find? a) (l₂.find? a) := by
+  match l₁, l₂ with
+  | ⟨.nil, _⟩, ⟨.nil, _⟩ => exact hf.symm
+  | ⟨.nil, _⟩, ⟨.cons x' y' t', h'⟩ =>
+    rw [merge_mk_nil_mk_cons, find?_filterMapVal, find?_mk_nil, Option.bind]
+    split <;> (rename_i w; rw [w])
+    rw [hf]
+  | ⟨.cons x y t, h⟩, ⟨.nil, _⟩ =>
+    rw [merge_mk_cons_mk_nil, find?_filterMapVal, find?_mk_nil, Option.bind]
+    split <;> (rename_i w; rw [w])
+    rw [hf]
+  | ⟨.cons x y t, h⟩, ⟨.cons x' y' t', h'⟩ =>
+    rw [merge_mk_cons_mk_cons]
+    split <;> rename_i h₁
+    · split <;> rename_i h₂
+      · rw [find?_merge hf]
+        rw [find?_mk_cons (a := x)]
+        split <;> rename_i h₃
+        · rcases AntisymmCmp.eq_of_cmp_eq h₃ with rfl
+          rw [find?_eq_none_of_ltHeadKey?, find?_eq_none_of_ltHeadKey?, hf]
+          · simp_all
+          · exact h₁
+          · exact AssocList.ltHeadKey?_of_keysOrdered_cons h
+        · rfl
+      · rw [find?_mk_cons]
+        split <;> rename_i h₃
+        · rcases AntisymmCmp.eq_of_cmp_eq h₃ with rfl
+          simp only [← h₂, find?_mk_cons_self]
+          rw [find?_eq_none_of_ltHeadKey?]
+          exact h₁
+        · rw [find?_merge hf, find?_mk_cons (a := x), if_neg h₃]
+    · rcases (AntisymmCmp.eq_of_cmp_eq h₁)
+      split <;> rename_i h₂
+      · rw [find?_merge hf]
+        rw [find?_mk_cons, find?_mk_cons]
+        split <;> rename_i h₃
+        · rcases (AntisymmCmp.eq_of_cmp_eq h₃)
+          rw [find?_eq_none_of_ltHeadKey?, find?_eq_none_of_ltHeadKey?, hf, h₂]
+          · exact AssocList.ltHeadKey?_of_keysOrdered_cons h'
+          · exact AssocList.ltHeadKey?_of_keysOrdered_cons h
+        · rfl
+      · rw [find?_mk_cons]
+        split <;> rename_i h₃
+        · rcases (AntisymmCmp.eq_of_cmp_eq h₃)
+          rw [find?_mk_cons_self, find?_mk_cons_self, h₂]
+        · rw [find?_merge hf, find?_mk_cons (a := x), if_neg h₃, find?_mk_cons (a := x), if_neg h₃]
+    · split <;> rename_i h₂
+      · rw [find?_merge hf]
+        rw [find?_mk_cons (a := x')]
+        split <;> rename_i h₃
+        · rcases (AntisymmCmp.eq_of_cmp_eq h₃)
+          rw [find?_eq_none_of_ltHeadKey?, find?_eq_none_of_ltHeadKey?, hf]
+          · exact h₂.symm
+          · exact AssocList.ltHeadKey?_of_keysOrdered_cons h'
+          · exact OrientedCmp.cmp_eq_gt.mp h₁
+        · rfl
+      · rw [find?_mk_cons]
+        split <;> rename_i h₃
+        · rcases (AntisymmCmp.eq_of_cmp_eq h₃)
+          simp only [find?_mk_cons_self]
+          rw [find?_eq_none_of_ltHeadKey?, h₂]
+          exact OrientedCmp.cmp_eq_gt.mp h₁
+        · rw [find?_merge hf, find?_mk_cons (a := x'), if_neg h₃]
+
+theorem merge_comm
+    (f : α → Option β → Option γ → Option δ) (g : α → Option γ → Option β → Option δ)
+    (hf : ∀ a, f a none none = none) (hg : ∀ a, g a none none = none)
+    (w : ∀ a x y, f a x y = g a y x)
+    (l₁ : OrderedAssocList cmp β) (l₂) : merge f l₁ l₂ = merge g l₂ l₁ := by
+  ext
+  simp [w, hf, hg]
+
+theorem merge_assoc
+    (f₁ : α → Option β₁ → Option β₂ → Option γ₁) (f₂ : α → Option γ₁ → Option β₃ → Option ε)
+    (g₁ : α → Option β₂ → Option β₃ → Option γ₂) (g₂ : α → Option β₁ → Option γ₂ → Option ε)
+    (hf₁ : ∀ a, f₁ a none none = none) (hf₂ : ∀ a, f₂ a none none = none)
+    (hg₁ : ∀ a, g₁ a none none = none) (hg₂ : ∀ a, g₂ a none none = none)
+    (w : ∀ a x y z, f₂ a (f₁ a x y) z = g₂ a x (g₁ a y z))
+    (l₁ : OrderedAssocList cmp β₁) (l₂) (l₃) :
+    merge f₂ (merge f₁ l₁ l₂) l₃ = merge g₂ l₁ (merge g₁ l₂ l₃) := by
+  ext
+  simp [w, hf₁, hf₂, hg₁, hg₂]
+
+/--
+Add two `OrderedAssocList`s, taking the value from one list if the other value is missing.
+(That is, treating missing values as `0`.)
+-/
+def add [Add β] (l₁ : OrderedAssocList cmp β) (l₂ : OrderedAssocList cmp β) :
+    OrderedAssocList cmp β :=
+  merge (fun _ => addOption) l₁ l₂
+where addOption : Option β → Option β → Option β
+  | some x, some y => some (x + y)
+  | some x, none => some x
+  | none, some y => some y
+  | none, none => none
+
+-- This statement will look better on the version of `OrderedAssocList` with default values,
+-- where we can just write `(add l₁ l₂).find a = l₁.find a + l₂.find a`.
+
+@[simp] theorem find?_add [Add β] {l₁ : OrderedAssocList cmp β} :
+    (add l₁ l₂).find? a =
+      match l₁.find? a, l₂.find? a with
+      | some x, some y => some (x + y)
+      | some x, none => some x
+      | none, some y => some y
+      | none, none => none := by
+  rw [add, find?_merge rfl]
+  rfl
+
+/--
+Multiply two `OrderedAssocList`s,
+dropping any values where the corresponding value in the other list is missing.
+(That is, treating missing values as `0`.)
+-/
+def mul [Mul β] (l₁ : OrderedAssocList cmp β) (l₂ : OrderedAssocList cmp β) :
+    OrderedAssocList cmp β :=
+  merge (fun _ => mulOption) l₁ l₂
+where mulOption : Option β → Option β → Option β
+  | some x, some y => some (x * y)
+  | some _, none => none
+  | none, some _ => none
+  | none, none => none
+
+@[simp] theorem find?_mul [Mul β] {l₁ : OrderedAssocList cmp β} :
+    (mul l₁ l₂).find? a =
+      match l₁.find? a, l₂.find? a with
+      | some x, some y => some (x * y)
+      | some _, none => none
+      | none, some _ => none
+      | none, none => none := by
+  rw [mul, find?_merge rfl]
+  rfl
+
+end merge
+
+end OrderedAssocList
